StandardAlgorithms/mutating/reverse/reverse.c
@@ -8,12 +8,12 @@ reverse(value_type* a, size_type n)
 {
   const size_type half = n / 2u;
 
-  //@ assert half: half <= n - half;
-  //@ assert half: 2*half <= n <= 2*half + 1;
+  //@ assert half:    half <= n - half;
+  //@ assert half:  2*half <= n <= 2*half + 1;
   /*@
     loop invariant bound:    0 <= i <= half <= n-i;
     loop invariant left:     Reverse{Pre,Here}(a, 0, i, n-i);
-    loop invariant middle: Unchanged{Pre,Here}(a, i, n-i);
+    loop invariant middle:   Unchanged{Pre,Here}(a, i, n-i);
     loop invariant right:    Reverse{Pre,Here}(a, n-i, n, 0);
     loop assigns i, a[0..n-1];
     loop variant half - i;
