StandardAlgorithms/mutating/rewrite_array_nothing/rewrite_array_nothing.c
@@ -1,0 +1,17 @@
+
+#include "rewrite_array_nothing.h"
+
+void rewrite_array(value_type* a, size_type n)
+{
+  /*@
+    loop invariant 0u <= i <= n;
+    loop invariant array_prefix: Unchanged{Pre,Here}(a, 0, i);
+    loop invariant array_suffix: Unchanged{Pre,Here}(a, i, n);
+    loop assigns i, a[0..n-1];
+    loop variant n - i;
+  */
+  for (size_type i = 0u; i < n; i++) {
+    a[i] = a[i];
+  }
+}
+
