StandardAlgorithms/mutating/rewrite_array_nothing/rewrite_array_nothing.h
@@ -1,0 +1,15 @@
+
+#ifndef REWRITE_ARRAY_H_INCLUDED
+#define REWRITE_ARRAY_H_INCLUDED
+
+#include "Unchanged.acsl"
+
+/*@
+  requires \valid(a + (0..n-1));
+  assigns  \nothing;
+  ensures  Unchanged{Pre,Post}(a,0,n);
+*/
+void rewrite_array(value_type* a, size_type n);
+
+#endif /* REWRITE_ARRAY_H_INCLUDED */
+
