StandardAlgorithms/mutating/rewrite_array_nothing/rewrite_array_nothing_test.cpp
@@ -1,0 +1,10 @@
+
+#include <iostream>
+
+int
+main(int argc, char** argv)
+{
+  std::cout << "\tsuccessful dummy test of " << argv[0] << std::endl;
+  return EXIT_SUCCESS;
+}
+
