StandardAlgorithms/mutating/rotate/rotate.h
@@ -2,22 +2,21 @@
 #ifndef ROTATE_H_INCLUDED
 #define ROTATE_H_INCLUDED
 
-#include "Equal.acsl"
+#include "Rotate.acsl"
 
 /*@
   requires   valid:   \valid(a + (0..n-1));
-  requires   bound:   m <= n;
+  requires   bound:   p <= n;
 
   terminates          \true;
   exits               \false;
   assigns             a[0..n-1];
 
-  ensures    result:  \result == n-m;
-  ensures    left:    Equal{Old,Here}(a, 0, m, n-m);
-  ensures    right:   Equal{Old,Here}(a, m, n, 0);
+  ensures    result:  \result == n-p;
+  ensures    rotate:  Rotate{Old,Here}(a, p, n);
 */
 size_type
-rotate(value_type* a, size_type m, size_type n);
+rotate(value_type* a, size_type p, size_type n);
 
 #endif  /* ROTATE_H_INCLUDED */
 
