StandardAlgorithms/mutating/rotate_copy/rotate_copy.h
@@ -2,11 +2,11 @@
 #ifndef ROTATE_COPY_H_INCLUDED
 #define ROTATE_COPY_H_INCLUDED
 
-#include "Equal.acsl"
+#include "Rotate.acsl"
 #include "Unchanged.acsl"
 
 /*@
-  requires   bound:      0 <= m <= n;
+  requires   bound:      0 <= p <= n;
   requires   valid:      \valid_read(a + (0..n-1));
   requires   valid:      \valid(b + (0..n-1));
   requires   sep:        \separated(a + (0..n-1), b + (0..n-1));
@@ -15,12 +15,11 @@
   exits                  \false;
   assigns                b[0..(n-1)];
 
-  ensures    left:       Equal{Old,Here}(a, 0, m,   b, n-m);
-  ensures    right:      Equal{Old,Here}(a, m, n-m, b, 0);
+  ensures    rotate:     Rotate{Old,Here}(a, p, n, b);
   ensures    unchanged:  Unchanged{Old,Here}(a, n);
 */
 void
-rotate_copy(const value_type* a, size_type m, size_type n, value_type* b);
+rotate_copy(const value_type* a, size_type p, size_type n, value_type* b);
 
 #endif /* ROTATE_COPY_H_INCLUDED */
 
